New SN proof for STLC

coq/LC/Debruijn/STLC.v
@@ -108,23 +108,30 @@ Lemma typing_varE ctx (n : nat) ty : (ctx \|- n \: ty) = ctxindex ctx n ty.
 Proof. by rewrite /typing /=. Qed.
 
 Lemma typing_appP ctx t1 t2 ty :
-  reflect (exists tyl, (ctx \|- t1 \: tyl :->: ty) && (ctx \|- t2 \: tyl))
+  reflect (exists2 tyl, (ctx \|- t1 \: tyl :->: ty) & (ctx \|- t2 \: tyl))
           (ctx \|- t1 @ t2 \: ty).
 Proof.
   apply: (iffP idP); rewrite /typing /=.
   - move: (typing_rec ctx t1) (typing_rec ctx t2) =>
       [] // [] // tyl tyr [] // tyl'; case: ifP => // /eqP <- /eqP [] ->.
     by exists tyl; rewrite !eqxx.
-  - by case => tyl /andP [] /eqP <- /eqP <-; rewrite eqxx.
+  - by case => tyl /eqP <- /eqP <-; rewrite eqxx.
 Qed.
 
 Lemma typing_absP ctx (t : term) tyl ty :
-  reflect (exists tyr, ty = (tyl :->: tyr) /\ Some tyl :: ctx \|- t \: tyr)
+  reflect (exists2 tyr, ty = (tyl :->: tyr) & Some tyl :: ctx \|- t \: tyr)
           (ctx \|- abs tyl t \: ty).
 Proof.
   apply: (iffP idP); rewrite /typing /=.
   - by case: typing_rec => //= tyr /eqP [] ->; exists tyr.
   - by case => tyr [] ->; case: typing_rec => // tyr' /eqP [] <-.
+Qed.
+
+Lemma typing_absE ctx (t : term) tyl tyr :
+  (ctx \|- abs tyl t \: tyl :->: tyr) = (Some tyl :: ctx \|- t \: tyr).
+Proof.
+  by rewrite /typing /=; case: typing_rec => //= tyr';
+    rewrite /eq_op /= /eq_op /= -/eq_op eqxx.
 Qed.
 
 Notation SN := (Acc (fun x y => betared1 y x)).
@@ -206,13 +213,13 @@ Lemma ctxleq_preserves_typing ctx1 ctx2 t ty :
 Proof.
   elim: t ty ctx1 ctx2 => /= [n | tl IHtl tr IHtr | tyl t IHt] ty ctx1 ctx2.
   - move/ctxleqP; apply.
-  - by move => H /typing_appP [tyl] /andP [H0 H1]; apply/typing_appP;
-      exists tyl; rewrite (IHtl _ _ _ H H0) (IHtr _ _ _ H H1).
-  - by move => H /typing_absP [tyr] [->] H0; apply/typing_absP;
-      exists tyr; split => //; move: H0; apply IHt; rewrite ctxleqE eqxx /=.
+  - by move => H /typing_appP [tyl H0 H1]; apply/typing_appP;
+      exists tyl; [apply (IHtl _ _ _ H) | apply (IHtr _ _ _ H)].
+  - by move => H /typing_absP [tyr -> H0]; rewrite typing_absE;
+      move: H0; apply IHt; rewrite ctxleqE eqxx.
 Qed.
 
-Lemma subject_shift t c ctx1 ctx2 :
+Lemma typing_shift t c ctx1 ctx2 :
   typing (ctxinsert ctx2 ctx1 c) (shift (size ctx2) c t) = typing ctx1 t.
 Proof.
   rewrite /typing.
@@ -230,9 +237,9 @@ Proof.
   elim: t ty n ctx => /= [m | tl IHtl tr IHtr | tyl t IHt] ty n ctx H.
   - rewrite /typing /= nth_insert !size_map => /eqP ->; elimif.
     + apply/eqP/esym; rewrite nth_default ?size_map /=; elimif_omega.
-    + rewrite !(nth_map (var 0, tyvar 0)) //.
-      move: {H0} (all_nthP (var 0, tyvar 0) H m H0).
-      rewrite -(subject_shift _ 0 _ (ctxinsert [::] (take n ctx) n))
+    + rewrite -/typing !(nth_map (var 0, tyvar 0)) //.
+      move: {H H0} (all_nthP (var 0, tyvar 0) H m H0).
+      rewrite -(typing_shift _ 0 _ (ctxinsert [::] (take n ctx) n))
               size_insert /= add0n size_take minnC minKn /insert take0
               sub0n take_minn minnn size_take minnE subKn ?leq_subr //=
               drop_take_nil drop0 cats0 -catA -{4}(cat_take_drop n ctx).
@@ -240,10 +247,9 @@ Proof.
       by case: (leqP' n (size ctx)) =>
         //= /ltnW /drop_oversize ->; rewrite cats0;
         apply/ctxleqP => /= n' ty' /eqP; rewrite nth_nseq if_same.
-  - by case/typing_appP => tyl /andP [] H0 H1; apply/typing_appP;
-      exists tyl; rewrite (IHtl _ _ _ H H0) (IHtr _ _ _ H H1).
-  - by case/typing_absP => tyr [] -> H0; apply/typing_absP;
-      exists tyr; split => //; apply IHt.
+  - by case/typing_appP => tyl H0 H1; apply/typing_appP; exists tyl;
+      [apply (IHtl _ _ _ H) | apply (IHtr _ _ _ H)].
+  - by case/typing_absP => tyr -> H0; rewrite typing_absE; apply IHt.
 Qed.
 
 Lemma subject_subst0 t ty ctx ctx' :
@@ -261,21 +267,23 @@ Theorem subject_reduction ctx t1 t2 ty :
   t1 ->b1 t2 -> ctx \|- t1 \: ty -> ctx \|- t2 \: ty.
 Proof.
   move => H; move: t1 t2 H ctx ty; refine (betared1_ind _ _ _ _) => /=.
-  - move => ty t1 t2 ctx ty2 /typing_appP [tyl] /andP []
-      /typing_absP [tyr] [] [] -> -> H H0.
+  - move => ty t1 t2 ctx ty2 /typing_appP [tyl] /typing_absP [tyr [-> ->]] H H0.
     by apply (subject_subst0 [:: (t2, ty)]) => //=; rewrite H0.
-  - by move => t1 t1' t2 H H0 ctx ty /typing_appP [tyl] /andP [H1 H2];
-      apply/typing_appP; exists tyl; rewrite H2 andbT; apply H0.
-  - by move => t1 t2 t2' H H0 ctx ty /typing_appP [tyl] /andP [H1 H2];
-      apply/typing_appP; exists tyl; rewrite H1 /=; apply H0.
-  - by move => tyl t t' H H0 ctx ty /typing_absP [tyr] [->] H1;
-      apply/typing_absP; exists tyr; split => //; apply H0.
+  - by move => t1 t1' t2 H H0 ctx ty /typing_appP [tyl H1 H2];
+      apply/typing_appP; exists tyl; [apply H0 | apply H2].
+  - by move => t1 t2 t2' H H0 ctx ty /typing_appP [tyl H1 H2];
+      apply/typing_appP; exists tyl; [apply H1 | apply H0].
+  - by move => tyl t t' H H0 ctx ty /typing_absP [tyr -> H1];
+      rewrite typing_absE; apply H0.
 Qed.
 
 Hint Resolve ctxleq_preserves_typing subject_subst subject_reduction.
 
 End subject_reduction_proof.
 
+(*******************************************************************************
+  Strong normalization proof with the type-free version of reducibility
+*******************************************************************************)
 Module strong_normalization_proof_typefree.
 
 Fixpoint reducible (ty : typ) (t : term) : Prop :=
@@ -342,10 +350,10 @@ Proof.
       apply CR3 => //; auto => t' H0; inversion H0.
     + case/eqP => ->; tauto.
     + by move => n H [_ H0]; apply IH.
-  - move => tl IHtl tr IHtr tyr ctx ctx' /typing_appP [tyl] /andP [H H0] H1.
+  - move => tl IHtl tr IHtr tyr ctx ctx' /typing_appP [tyl H H0] H1.
     by move: (IHtl (tyl :->: tyr) ctx ctx') => /=;
       apply => //; apply IHtr with ctx.
-  - move => tyl t IHt ty ctx ctx' /typing_absP [tyr] [->] H H0.
+  - move => tyl t IHt ty ctx ctx' /typing_absP [tyr -> H] H0.
     simpl substitute; apply abstraction_lemma => t' H1.
     by rewrite subst_app /=; apply (IHt tyr ctx ((t', tyl) :: ctx')).
 Qed.
@@ -357,7 +365,10 @@ Qed.
 
 End strong_normalization_proof_typefree.
 
-Module strong_normalization_proof_typed.
+(*******************************************************************************
+  Strong normalization proof with the Kripke-style reducibility
+*******************************************************************************)
+Module strong_normalization_proof_kripke.
 
 Import subject_reduction_proof.
 
@@ -397,7 +408,7 @@ Proof.
   split => [ctx t H H0 | ctx tl H H0 H1 tr ctx' H2 H3 H4].
   - set H1 := ctxindex_last ctx tyl.
     have H2: ctx ++ [:: Some tyl] \|- t @ size ctx \: tyr by
-      apply/typing_appP; exists tyl; rewrite H1 andbT; eauto.
+      apply/typing_appP; exists tyl; eauto.
     suff: SN ([fun t => t @ size ctx] t) by
       apply acc_preservation; constructor.
     apply (IHtyr1 _ _ H2), IHtyr2 => // t' H3.
@@ -405,8 +416,7 @@ Proof.
     apply IHtyl2 => // x H4; inversion H4.
   - have H5: SN tr by apply IHtyl1 with ctx'.
     move: tr H5 H2 H3 H4; refine (Acc_ind _ _) => tr _ IH H2 H3 H4.
-    have H5: ctx' \|- tl @ tr \: tyr by
-      apply/typing_appP; exists tyl; rewrite H3 andbT; eauto.
+    have H5: ctx' \|- tl @ tr \: tyr by apply/typing_appP; exists tyl; eauto.
     apply IHtyr2 => // t' H6.
     move: H0; inversion H6; subst => // _; eauto.
 Qed.
@@ -423,15 +433,14 @@ Proof.
   move => /= H H0 t' ctx' H1 H2 H3.
   move: t' {H2 H3} (CR1 H2 H3) (H2) (H3); refine (Acc_ind _ _) => t' _ H2 H3 H4.
   have H5: ctx' \|- substitute 0 [:: t'] t \: tyr by
-    apply (subject_subst0 [:: (t', tyl)]); rewrite /= ?H3 //;
-      case/typing_absP: H => tyr' [] [] <-;
-      apply ctxleq_preserves_typing; rewrite ctxleqE eqxx.
+    apply (subject_subst0 [:: (t', tyl)]); rewrite /= ?H3 // -typing_absE;
+      move: H; apply ctxleq_preserves_typing.
   have {H5} H5: SN t by
     move: (CR1 H5 (H0 t' ctx' H1 H3 H4));
       apply acc_preservation => x y; apply subst_betared1.
   move: t H5 H H0 H2; refine (Acc_ind _ _) => t _ H H0 H2 H5; apply CR3 => //=.
-  - by apply/typing_appP; exists tyl; rewrite H3 andbT;
-      move: H0; apply ctxleq_preserves_typing.
+  - apply/typing_appP; exists tyl; last apply H3.
+    by move: H0; apply ctxleq_preserves_typing.
   - move => t'' H6.
     inversion H6; subst => {H6}; eauto.
     inversion H10; subst => {H10}; eauto.
@@ -453,18 +462,17 @@ Proof.
       apply CR3 => //; auto => t' H0; inversion H0.
     + case/eqP => ->; tauto.
     + by move => n H /andP [_ H0] [_]; apply IH.
-  - move => tl IHtl tr IHtr tyr ctx ctx' /typing_appP [tyl] /andP [H H0] H1 H2.
+  - move => tl IHtl tr IHtr tyr ctx ctx' /typing_appP [tyl H H0] H1 H2.
     move: (IHtl (tyl :->: tyr) ctx ctx') => /=; apply; auto.
     by apply subject_subst0.
-  - move => tyl t IHt ty ctx ctx' /typing_absP [tyr] [->] H H0 H1.
+  - move => tyl t IHt ty ctx ctx' /typing_absP [tyr -> H] H0 H1.
     simpl substitute; apply abstraction_lemma;
-      first by apply (@subject_subst0 (abs tyl t)) => //;
-        apply/typing_absP; exists tyr; split.
-    move => t2 ctx2 H2 H3 H4.
+      first by apply (@subject_subst0 (abs tyl t)) => //; rewrite typing_absE.
+    move => /= t2 ctx2 H2 H3 H4.
     rewrite subst_app /=.
     apply (IHt tyr ctx2 ((t2, tyl) :: ctx')) => /=.
-    + move: H; apply ctxleq_preserves_typing.
-      by rewrite ctxleqE eqxx ctxleq_appl /=.
+    + by move: H; rewrite -!typing_absE;
+        apply ctxleq_preserves_typing; rewrite ctxleq_appl.
     + rewrite H3 /=; move: H0; apply sub_all => p; eauto.
     + split => //; move: H1; apply Forall_impl; eauto.
 Qed.
@@ -473,6 +481,88 @@ Theorem typed_term_is_sn ctx t ty : ctx \|- t \: ty -> SN t.
 Proof.
   move => H; move: (@reduce_lemma ctx [::] _ _ H) => /= /(_ erefl I).
   by rewrite subst_nil; apply CR1.
+Qed.
+
+End strong_normalization_proof_kripke.
+
+(*******************************************************************************
+  Strong normalization proof with the typed version of reducibility (incomplete)
+*******************************************************************************)
+Module strong_normalization_proof_typed.
+
+Import subject_reduction_proof.
+
+Fixpoint list_hyp ty : seq typ :=
+  if ty is tyl :->: tyr then tyl :: list_hyp tyl ++ list_hyp tyr else [::].
+
+Fixpoint reducible (ctx : context typ) (ty : typ) (t : term) : Prop :=
+  match ty with
+    | tyvar n => SN t
+    | tyl :->: tyr => forall t',
+        ctx \|- t' \: tyl -> reducible ctx tyl t' -> reducible ctx tyr (t @ t')
+  end.
+
+Lemma CR2 ctx t t' ty :
+  t ->b1 t' -> reducible ctx ty t -> reducible ctx ty t'.
+Proof.
+  elim: ty ctx t t'.
+  - by move => /= _ _ t t' H []; apply.
+  - move => /= tyl IHtyl tyr IHtyr ctx t1 t2 H H0 t3 H1 H2.
+    by apply IHtyr with (t1 @ t3); auto.
+Qed.
+
+Hint Resolve CR2.
+
+Lemma CR1_and_CR3 ty :
+  (forall (ctx : context typ) t,
+   all (fun ty => Some ty \in ctx) (list_hyp ty) ->
+   ctx \|- t \: ty -> reducible ctx ty t -> SN t) /\
+  (forall ctx t,
+   all (fun ty => Some ty \in ctx) (list_hyp ty) ->
+   ctx \|- t \: ty -> neutral t ->
+   (forall t', t ->b1 t' -> reducible ctx ty t') -> reducible ctx ty t).
+Proof.
+  elim: ty; first by [].
+  move => /= tyl [IHtyl1 IHtyl2] tyr [IHtyr1 IHtyr2]; split => ctx tl.
+  - case/andP => /(nthP None) [x _] /esym /eqP H;
+      rewrite all_cat; case/andP => H0 H1 H2 H3.
+    have H4: ctx \|- tl @ x \: tyr by apply/typing_appP; exists tyl.
+    suff: SN ([fun t => t @ x] tl) by apply acc_preservation; constructor.
+    by apply (IHtyr1 ctx) => //; apply IHtyr2 => // t' H5;
+      apply (CR2 H5); apply H3 => //; apply IHtyl2 => // y H6; inversion H6.
+  - case/andP => _; rewrite all_cat; case/andP => H H0 H1 H2 H3 tr H4 H5.
+    have H6: SN tr by apply (IHtyl1 ctx).
+    move: tr H6 H4 H5; refine (Acc_ind _ _) => tr _ IH H4 H5.
+    have H6: ctx \|- tl @ tr \: tyr by apply/typing_appP; exists tyl.
+    apply IHtyr2 => // t' H7; move: H2; inversion H7; subst => // _; eauto.
+Qed.
+
+Definition CR1 t ty := proj1 (CR1_and_CR3 ty) t.
+Definition CR3 t ty := proj2 (CR1_and_CR3 ty) t.
+
+Lemma abstraction_lemma (ctx : context typ) t tyl tyr :
+  all (fun ty => Some ty \in ctx) (list_hyp (tyl :->: tyr)) ->
+  ctx \|- abs tyl t \: tyl :->: tyr ->
+  (forall t', ctx \|- t' \: tyl ->
+   reducible ctx tyl t' -> reducible ctx tyr (substitute 0 [:: t'] t)) ->
+  reducible ctx (tyl :->: tyr) (abs tyl t).
+Proof.
+  move => /= /andP [] H; rewrite all_cat; case/andP => H0 H1 H2 H3 t' H4 H5.
+  move: t' {H4 H5} (CR1 H0 H4 H5) (H4) (H5);
+    refine (Acc_ind _ _) => t' _ H4 H5 H6.
+  have H7: ctx \|- substitute 0 [:: t'] t \: tyr by
+    apply (subject_subst0 [:: (t', tyl)]); rewrite /= ?H5 // -typing_absE.
+  have {H7} H7: SN t by
+    move: (CR1 H1 H7 (H3 t' H5 H6));
+      apply acc_preservation => x y; apply subst_betared1.
+  move: t H7 H2 H3 H4; refine (Acc_ind _ _) => t _ H2 H3 H4 H7;
+    apply CR3 => //=.
+  - by apply/typing_appP; exists tyl.
+  - move => t'' H8.
+    inversion H8; subst => {H8}; eauto.
+    inversion H12; subst => {H12}; eauto.
+    apply H2 => //; eauto => t'' ctx'' H8.
+    by apply (CR2 (subst_betared1 0 [:: t''] H11)), H4.
 Qed.
 
 End strong_normalization_proof_typed.
